Test/VProg.v
@@ -10,7 +10,7 @@ Import VProg._Abbrev.
 
 Definition f_main : fid := 0.
 
-Definition sig_main := mk_f_sig (ptr * ptr) ptr.
+Definition sig_main := mk_f_sig (ptr * ptr * ptr) ptr.
 
 Definition SIG : sig_context :=
   fun f => match f with
@@ -18,81 +18,83 @@ Definition SIG : sig_context :=
   | _ => None
   end.
 
-Definition spec_main_n (ps : ptr * ptr) : SP.Spec.t ptr :=
-  let (p0, p1) := ps in {|
-  SP.Spec.pre  := SLprop.ex nat (fun n0 => SLprop.cell p0 n0) **
-                  SLprop.ex nat (fun n1 => SLprop.cell p1 n1);
-  SP.Spec.post := fun p => (SLprop.ex nat (fun n => SLprop.cell p n) ** SLprop.True)%slprop;
-|}.
-
-Definition spec_main : SP.f_spec sig_main :=
-  fun ps s => eq s (spec_main_n ps).
+Definition spec_main : f_spec sig_main :=
+  fun '(p0, p1, p2) =>
+  Spec.mk_r0 (fun '(n0, n1, n2) =>
+  Spec.mk_r1 [CTX.mka (SLprop.cell p2, n2)]
+             [CTX.mka (SLprop.cell p0, n0); CTX.mka (SLprop.cell p1, n1)] True (fun p =>
+  Spec.mk_r2 (fun '(n, n1') =>
+  Spec.mk_r3 [CTX.mka (SLprop.cell p, n); CTX.mka (SLprop.cell p1, n1')] (n1' > 0)))).
 
 Definition SPEC : CP.spec_context SIG :=
   fun f => match f with
-  | 0 => SP.tr_f_spec spec_main
+  | 0 => SP.tr_f_spec (tr_f_spec spec_main)
   | _ => tt
   end.
 
 Definition data42 : nat := 42.
 
-Definition vprog_main (ps : ptr * ptr) : instr SPEC ptr :=
-  let (p0, p1) := ps in
+Definition vprog_main (ps : ptr * ptr * ptr) : instr SPEC ptr :=
+  let '(p0, p1, p2) := ps in
   Bind _ (Read  _ p0) (fun v0 =>
   Bind _ (Write _ p1 data42) (fun _ =>
-  Bind _ (Assert _ [_] (fun '(v1,_) => ([CTX.mka (SLprop.cell p0,  v1)], v1 = v0))) (fun _ =>
+  Bind _ (Assert _ (fun '(v0', v1') =>
+    ([CTX.mka (SLprop.cell p0, v0'); CTX.mka (SLprop.cell p1, v1')], v0' = v0))) (fun _ =>
   Ret _ p0 (fun p => [Vprop.mk (SLprop.cell p)])))).
 
-Definition impl_main (ps : ptr * ptr) :
+Definition impl_main (ps : ptr * ptr * ptr) :
   { i : CP.instr ptr | i = i_impl (vprog_main ps) }.
 Proof.
   unfold i_impl, vprog_main; cbn.
-  case ps as (p, p0); cbn.
+  case ps as ((p0, p1), p2); cbn.
   eexists. reflexivity.
 Defined.
 
-Lemma sls_main (ps : ptr * ptr):
-  SP.sls SPEC (proj1_sig (impl_main ps)) (spec_main_n ps).
+Lemma imatch_main (ps : ptr * ptr * ptr):
+  impl_match SPEC (vprog_main ps) (spec_main ps).
 Proof.
-  case impl_main as [? ->]; simpl.
-  case ps as (p0, p1).
-  unfold spec_main_n; SP.normalize.
-  apply SP.ExistsE; intro v0.
-  apply SP.ExistsE; intro v1.
-  eapply SP.Cons.
-  - eapply (proj2_sig (i_spec (vprog_main _) [CTX.mka (SLprop.cell p0, v0); CTX.mka (SLprop.cell p1, v1)]))
-      with (post := fun _ => True).
-    + Tac.build_spec.
+  case ps as ((p0, p1), p2).
+  Tac.build_impl_match.
+  (*
+  apply intro_impl_match1.
+  cbn.
+  intros ((n0, n1), n2).
+  (* apply Impl_MatchI. (* Coq 8.15.2 BUG: Anomaly "in retyping: unbound local variable." *) *)
+  simple refine (@Impl_MatchI _ _ _ _ _ _ _ _ _ _ _ _ _ _ _ _ _ _ _ _ _).
+  1,2,3,4, 6,8,10,12:shelve.
+  - (* sel1_TU_GOAL *)
+    cbn; do 2 intro (* x sel1 *).
+    Tuple.build_type_iso_tu.
+  - (* F0      *) cbn. Tac.build_spec.
+  - (* F       *) Tac.cbn_refl.
+  - (* S_VPOST *) Tac.cbn_refl.
+  - (* EX_SEL1 *)
+    cbn; repeat intro.
+    Tac.simplify_ex_eq_tuple.
     (*
-    + Tac.build_Bind_init.
-      { Tac.build_Read. }
-      { Tac.cbn_refl. }
-      cbn; repeat intro.
-      Tac.build_Bind_init.
-      { Tac.build_Write. }
-      { Tac.cbn_refl. }
-      cbn; repeat intro.
-      Tac.build_Bind_init.
-      { Tac.build_Assert. }
-      { Tac.cbn_refl. }
-      cbn; repeat intro.
-      { simple refine (@Ret_SpecI _ _ _ _ _ _ _).
-        Tuple.build_shape.
-        shelve.
-        CTX.Inj.build. }
-      Tac.cbn_refl. Tac.cbn_refl. Tac.cbn_refl. Tac.cbn_refl.
-      Tac.cbn_refl. Tac.cbn_refl. Tac.cbn_refl. Tac.cbn_refl.
-      Tac.cbn_refl. Tac.cbn_refl. Tac.cbn_refl. Tac.cbn_refl.
+    etransitivity.
+    + etransitivity.
+      refine (exists_eq_const _ _ (fun x => _)).
+        refine (ex_ind (fun x => _)).
+        refine (VProg.Tac.elim_tuple_eq_conj _).
+        cbn; repeat intro; eassumption.
+      refine (exists_eq_const _ _ (fun x => _)).
+        refine (VProg.Tac.elim_tuple_eq_conj _).
+        cbn; repeat intro; eassumption.
+    + refine (VProg.Tac.simpl_tuple_eq_conj _ _).
+      * cbn.
+        refine (simpl_and_list_r1 eq_refl _).
+        refine (simpl_and_list_r1 eq_refl _).
+        refine (simpl_and_list_e1 _).
+        exact simpl_and_list_0.
+      * cbn; reflexivity.
     *)
-    + unfold FP.BindA. cbn. auto.
-  - cbn.
-    split; cbn.
-    + SLprop.normalize. reflexivity.
-    + clear; intro p.
-      apply SLprop.imp_exists_l; intros (v, (?, [])).
-      apply SLprop.imp_pure_l;   intros _.
-      apply SLprop.imp_exists_r with (wit := v).
-      apply SLprop.star_morph_imp.
-      reflexivity.
-      constructor.
+  - (* rsel    *) cbn; repeat intro. Tuple.build_shape.
+  - (* RSEL    *) cbn; repeat intro. CTX.Inj.build.
+  *)
+  - (* WLP *)
+    cbn.
+    unfold FP.BindA; cbn.
+    intuition.
+    unfold data42; repeat constructor.
 Qed.
